base-thy/Control/Concurrency/Interp.v
@@ -1,0 +1,97 @@
+Require Import GHC.MVar.
+Require Import Control.Concurrent.MVar.
+
+Require Import Streams Arith.
+
+Open Scope nat_scope.
+
+Record heap :=
+  { max_loc : nat;
+    content : nat -> option nat }.
+
+Definition empty_heap :=
+  {| max_loc := 0;
+     content := fun _ => None |}.
+
+Definition prog := IO unit.
+
+Inductive stopFlag :=
+| Unexpected
+| Blocked
+| Finished.
+
+Program Definition interp (p : prog) (h : heap) : (stopFlag + (prog * heap)) :=
+  match p with
+  | GHC.IO.Ret m => inl Finished
+  | GHC.IO.Vis eff k => _
+  end.
+Next Obligation.
+  destruct eff eqn:Heff.
+  - destruct h.
+    remember (max_loc0 + 1) as max_loc1. right.
+    exact (k (MkMV max_loc1),
+           {| max_loc := max_loc1;
+              content := fun n => if (n =? max_loc0) then None else content0 n
+           |}).
+  - destruct m.
+    destruct (content h loc) eqn:Hcontent.
+    + destruct (@decode A _ n) eqn:Hdecode.
+      * right. destruct h.
+        exact (k a,
+               {| max_loc := max_loc0;
+                  content := fun n => if n =? loc then None else content0 n
+               |}).
+      * left. exact Unexpected.
+    + left. exact Blocked.
+  - destruct m.
+    destruct (content h loc) eqn:Hcontent.
+    + destruct (@decode A _ n) eqn:Hdecode.
+      * right. exact (k a, h).
+      * left. exact Unexpected.
+    + left. exact Blocked.
+  - destruct m.
+    destruct (content h loc) eqn:Hcontent.
+    + left. exact Blocked.
+    + right. destruct h.
+      exact (k tt,
+             {| max_loc := max_loc0;
+                content := fun n => if n =? loc then (Some (encode a))  else content0 n
+             |}).
+  - destruct m.
+    destruct (content h loc) eqn:Hcontent.
+    + destruct (@decode A _ n) eqn:Hdecode.
+      * right. destruct h.
+        exact (k (Some a),
+               {| max_loc := max_loc0;
+                  content := fun n => if n =? loc then None else content0 n
+               |}).
+      * left. exact Unexpected.
+    + right. exact (k None, h).
+  - destruct m.
+    destruct (content h loc) eqn:Hcontent.
+    + destruct (@decode A _ n) eqn:Hdecode.
+      * right. exact (k (Some a), h).
+      * left. exact Unexpected.
+    + right. exact (k None, h).
+  - destruct m.
+    destruct (content h loc) eqn:Hcontent.
+    + right. exact (k false, h).
+    + right. destruct h.
+      exact (k true,
+             {| max_loc := max_loc0;
+                content := fun n => if n =? loc then (Some (encode a))  else content0 n
+             |}).
+  - destruct m.
+    destruct (content h loc) eqn:Hcontent.
+    + right. exact (k false, h).
+    + right. exact (k true, h).
+Defined.
+
+Inductive safe_single_prog_on_heap (p : prog) (h : heap) : Prop :=
+| SafeFinished (_ : interp p h = inl Finished)
+| SafeRunning : forall p' h', interp p h = inr (p', h') ->
+                         safe_single_prog_on_heap p' h' ->
+                         safe_single_prog_on_heap p h.
+
+Definition safe_single_prog (p : prog) : Prop :=
+  safe_single_prog_on_heap p empty_heap.
